# 几个常用的展开式

$$
\begin{flalign*}
	&(1)\quad
	e^x
	=1+x+\frac{x^2}{2}+\cdots+\frac{x^n}{n!}+\cdots
	=\sum\limits_{n=0}^{\infty}\frac{x^n}{n!}
	\qquad (-\infty< x< +\infty)
	\newline
	&(2)\quad
	\sin x
	=x-\frac{x^3}{3}+\cdots+\frac{(-1)^{n-1}x^{2n-1}}{(2n-1)!}+\cdots
	=\sum\limits_{n=0}^{\infty}\frac{(-1)^nx^{2n+1}}{(2n+1)!}
	\qquad (-\infty< x< +\infty)\newline
	&(3)\quad
	\cos x
	=1-\frac{x^2}{2}+\cdots+\frac{(-1)^{n}x^{2n}}{(2n)!}+\cdots
	=\sum\limits_{n=1}^{\infty}\frac{(-1)^nx^{2n}}{(2n)!}
	\qquad (-\infty< x< +\infty)\newline
	&(4)\quad
	(x+1)^\alpha
	=1+\alpha x+\frac{\alpha(\alpha-1)}{2!}x^2+\cdots+\frac{\alpha(\alpha-1)\cdots(\alpha-n+1)}{n!}x^n+\cdots
	=\sum\limits_{n=0}^{\infty}\frac{\alpha(\alpha-1)\cdots(\alpha-n+1)}{n!}x^n
	\qquad (-1< x< 1)\newline
	&(5)\quad
	\ln (x+1)
	=x-\frac{x^2}{2}+\cdots+\frac{(-1)^{n-1}x^{n}}{n}+\cdots
	=\sum\limits_{n=1}^{\infty}\frac{(-1)^{n-1}x^n}{n}
	\qquad (-1< x\leqslant 1)\newline
	&(6)\quad
	-\ln(1-x)
	=x+\frac{x^2}{2}+\cdots+\frac{x^n}{n}+\cdots
	=\sum_{n=1}^{∞}\frac{x^n}{n}
	\qquad (-1\leqslant x<1)\newline
	&(7)\quad
	\frac{1}{1-x}
	=1+x+\cdots+x^n+\cdots
	=\sum\limits_{n=0}^{\infty}x^n
	\qquad (-1< x< 1)\newline
	&(8)\quad
	\frac{1}{1+x}
	=1-x+\cdots+(-1)^nx^n+\cdots
	=\sum\limits_{n=0}^{\infty}(-1)^nx^n
	\qquad (-1< x< 1)\newline
\end{flalign*}
$$
