### 柯西定理

若$f(x),g(x)$

1. 在$[a,b]$上连续;
2. 在$(a,b)$内可导;
3. 且$\forall x \in (a,b), g'(x)\not=0$;

那么至少存在一个$\xi\in (a, b)$, 使
$$\frac{f(b)-f(a)}{g(b)-g(a)}=\frac{f'(\xi)}{g'(\xi)}$$

#### 证明柯西定理

$$
\begin{aligned}
	& 由拉格朗日中值定理知, \exists \eta\in (a,b), g(b)-g(a)=g'(\eta)(b-a)\\
	& 又g'(x)\not= 0, \therefore g(b)- g(a)\not= 0\\
	& 设辅助函数\\
	& \qquad\varphi (x)= f(x)- \frac{f(b)-f(a)}{g(b)-g(a)}g(x)\\
	& 显然, \varphi (x)在闭区间[a,b]连续, 开区间(a,b)可导\\
	& 且\varphi(a)= \varphi(b)= \frac{g(b)f(a)-g(a)f(b)}{g(b)-g(a)}\\
	& 根据罗尔定理知, \exists \xi \in (a,b),使\varphi'(\xi)=0\\
	& 即\frac{f(b)-f(a)}{g(b)-g(a)}=\frac{f'(\xi)}{g'(\xi)}\\
	\newline
	& 要证 [f(b)-f(a)]g'(\xi)-[g(b)-g(a)]f'(\xi)=0\\
	& 1)\ F(x)=[f(b)-f(a)]g(x)-[g(b)-g(a)]f(x) \quad F(a)=F(b)\\
	& 2)\ F(x)=[f(b)-f(a)][g(x)-g(a)]-[g(b)-g(a)][f(x)-f(b)] \quad F(a)=F(b)\\
\end{aligned}
$$
