# 矩阵的乘法

$$
\begin{aligned}
	& \pmb{A}_{m\times s}, \pmb{B}_{s\times n}\\
	& \pmb{C}=\pmb{A}\pmb{B}=[c_{ij}]_{m\times n} \\
	& \boxed{c_{ij}=\sum\limits_{k=1}^{s}a_{ik}b_{kj}}\\
\end{aligned}
$$

## <font color=red>注</font>

- $\pmb{A}$列数= $\pmb{B}$行数
- $\pmb{C}$行数= $\pmb{A}$行数, $\pmb{C}$列数=$\pmb{B}$列数

## 运算律

一般不满足:

- 交换率 $\pmb{A}\pmb{B}\not=\pmb{B}\pmb{A}$
- 消去律 $\pmb{A}\pmb{B}=\pmb{O} \nRightarrow \pmb{A}=\pmb{O}或\pmb{B}=\pmb{O}; \pmb{A}\pmb{B}=\pmb{A}\pmb{C}且\pmb{A}\not=\pmb{O} \nRightarrow \pmb{B}=\pmb{C}$,

若两方阵满足$\pmb{A}\pmb{B}=\pmb{B}\pmb{A}$, 称方阵$\pmb{A}, \pmb{B}$<b>可交换</b>

满足:

- 结合律: $(\pmb{A}\pmb{B})\pmb{C}=\pmb{A}(\pmb{B}\pmb{C})$,
- 数乘结合律: $\lambda(\pmb{A}\pmb{B})= (\lambda \pmb{A})\pmb{B}= \pmb{A} (\lambda \pmb{B})$,
- 分配率: $\pmb{A}(\pmb{B}+\pmb{C})= \pmb{A}\pmb{B}+\pmb{A}\pmb{C}, (\pmb{B}+\pmb{C})\pmb{A}=\pmb{B}\pmb{A}+ \pmb{C}\pmb{A}$.
- $\pmb{A}_{m\times p} \cdot \pmb{O}_{p\times n}= \pmb{O}_{m\times n} \qquad \pmb{O}_{k\times m}\cdot \pmb{A}_{m\times p}= \pmb{O}_{k\times p}$

> 矩阵的幂也满足上述三律

## 单位矩阵/纯量阵与矩阵的乘积

$$
\begin{aligned}
	& \pmb{E}_m\pmb{A}_{m\times n}=\pmb{A}_{m\times n} \qquad \pmb{A}_{m\times n}\pmb{E}_n=\pmb{A}_{m\times n}\\
	& \pmb{E}\pmb{A}=\pmb{A}\pmb{E}=\pmb{A}
\end{aligned}
$$

纯量阵:

$$
\begin{aligned}
	&
	\lambda \pmb{E} =
	\begin{pmatrix}
		\lambda & & &\\
		& \lambda & &\\
		& & \ddots & \\
		& & & \lambda
	\end{pmatrix}\\
	& (\lambda \pmb{E})\pmb{A} = \lambda \pmb{A}, \pmb{A}(\lambda \pmb{E})= \lambda \pmb{A}\\
	& 当\pmb{A}为方阵时, 有
	(\lambda \pmb{E}_n)\pmb{A}_n = \lambda \pmb{A}_n= \pmb{A}_n(\lambda \pmb{E}_n)
\end{aligned}
$$

## 对角矩阵的乘法

$$
\begin{aligned}
	& \pmb{\Lambda}=\mathrm{diag}(a_1, a_2, \dots, a_n)\\
	&
	\begin{pmatrix}
		a_1 & 0 & 0\\
		0 & a_2 & 0\\
		0 & 0 & a_3
	\end{pmatrix}
	\begin{pmatrix}
		b_1 & 0 & 0\\
		0 & b_2 & 0\\
		0 & 0 & b_3
	\end{pmatrix}=
	\begin{pmatrix}
		a_1b_1 & 0 & 0\\
		0 & a_2b_2 & 0\\
		0 & 0 & a_3b_3
	\end{pmatrix}\\
\end{aligned}
$$

### 一些性质:

$$
\begin{aligned}
	& (1)\ \pmb{\Lambda_1\Lambda_2}=\pmb{\Lambda_2\Lambda_1}\\
	& (2)\
	\begin{pmatrix}
		a_1 & 0 & 0\\
		0 & a_2 & 0\\
		0 & 0 & a_3
	\end{pmatrix}^n=
	\begin{pmatrix}
		a_1^n & 0 & 0\\
		0 & a_2^n & 0\\
		0 & 0 & a_3^n
	\end{pmatrix}\\
	& (3)\
	\begin{pmatrix}
		a_1 & 0 & 0\\
		0 & a_2 & 0\\
		0 & 0 & a_3
	\end{pmatrix}^{-1}=
	\begin{pmatrix}
		\frac{1}{a_1} & 0 & 0\\
		0 & \frac{1}{a_2} & 0\\
		0 & 0 & \frac{1}{a_3}
	\end{pmatrix}
\end{aligned}
$$
