## 题

$$
\begin{aligned}
	& 设a_n= \int_{0}^{1} x^n \sqrt[]{1-x^2}\mathrm{d}x(n=1, 2, 3 \dots)\\
	& (1)\ 证明: 数列 \{a_n\} 单调递减, 且a_n= \frac{n-1}{n+2}\cdot a_{n-2}( n=2, 3\dots)\\
	& (2)\ \lim\limits_{n\to \infty} \frac{a_n}{a_{n-1}}.
\end{aligned}
$$

## 解

$$
\begin{aligned}
	& (1)\\
	& \text{When}\ x \in [0, 1], x^{n+1}\sqrt[]{1-x^2} \leqslant x^n \sqrt[]{1-x^2}\\
	& \therefore \int_{0}^{1} x^{n+1}\sqrt[]{1-x^2}\mathrm{d}x < x^{n}\sqrt[]{1-x^2}\mathrm{d}x\\
	& 即 a_{n+1}< a_n, 数列 \{a_n\} 单调递减\\
	& 方法1:\\
	&
\begin{equation}
\begin{split}
	a_n
	&= \int_{0}^{1} x^{n-1}x \sqrt[]{1-x^2}\mathrm{d}x \\
	&= -\frac{1}{2}\int_{0}^{1} x^{n-1} \sqrt[]{1-x^2}\mathrm{d}(1-x^2) \\
	&= -\frac{1}{2} \frac{2}{3}\int_{0}^{1} x^{n-1} \mathrm{d}(1-x^2)^{\frac{3}{2}} \\
	&= -\frac{1}{3}x^{n-1}(1-x^2)^{\frac{3}{2}} \bigg|_0^1 + \frac{1}{3} \int_{0}^{1} (1-x^2)^{\frac{3}{2}} (n-1)x^{n-2}\mathrm{d}x\\
	&= \frac{n-1}{3} \int_{0}^{1} (x^{n-2} - x^n)\sqrt[]{1-x^2}\mathrm{d}x\\
	& = \frac{n-1}{3}(a_{n-2} + a_n)
\end{split}
\end{equation}\\
	& 解得a_n= \frac{n-1}{n+2}a_{n-2}\\
\end{aligned}
$$

$$
\begin{aligned}
	& 方法2:\\
	& 令x= \sin t, 则t\in (0, \frac{\pi}{2})\\
	&
	\begin{equation}
	\begin{split}
		a_n
		&= \int_{0}^{1} x^n\sqrt[]{1-x^2}\mathrm{d}x\\
		&= \int_{0}^{\frac{\pi}{2}} \sin^n t \cos^2 t\mathrm{d}t\\
		&= \int_{0}^{\frac{\pi}{2}} \sin^n t - \sin^{n+2} t\mathrm{d}t\\
		a_{n-2}
		&= \int_{0}^{1} x^{n-2}\sqrt[]{1-x^2}\mathrm{d}x\\
		&= \int_{0}^{\frac{\pi}{2}} \sin^{n-2} t \cos^2 t\mathrm{d}t\\
		&= \int_{0}^{\frac{\pi}{2}} \sin^{n-2} t - \sin^{n} t\mathrm{d}t\\
		令I_n
		&= \int_{0}^{\frac{\pi}{2}} \sin^n t\mathrm{d}t\\
		&= \int_{0}^{\frac{\pi}{2}} \sin^{n-1} t\mathrm{d}(-\cos t)\\
		&= -\cos t \sin^{n-1} t\bigg|_0^{\frac{\pi}{2}}+ \int_{0}^{\frac{\pi}{2}} \cos t\mathrm{d}x (\sin^{n-1} t)\\
		&= (n-1)\int_{0}^{\frac{\pi}{2}} \sin^{n-2}t \cos^2 t\mathrm{d}t\\
		&= (n-1)\int_{0}^{\frac{\pi}{2}} \sin^{n-2}t - \sin^n t\mathrm{d}t\\
		&= (n-1)(I_{n-2}- I_n)\\
		I_n
		&= \frac{n-1}{n}I_{n-2}\\
	\end{split}
	\end{equation}\\
	&	a_n= I_n-I_{n+2}= \frac{1}{n+2}I_n\\
	& a_{n-2}= I_{n-2}- I_n= \frac{1}{n-1}I_n\\
	& \therefore a_{n} = \frac{n-1}{n+2}a_{n-2}
\end{aligned}
$$

$$
\begin{aligned}
	& (2)\\
	& \because a_{n}单调递减,\\
	& \therefore a_{n-1}> a_n= \frac{n-1}{n+2}a_{n-2} > \frac{n-1}{n+2}a_{n-1}\\
	& \therefore 1> \frac{a_n}{a_{n-1}}> \frac{n-1}{n+2}\\
	& 由夹逼定理知极限为1.
\end{aligned}
$$

## 知识点

- ![[夹逼准则]]
- 积分换元法![[三种主要积分法#2. 第二类换元法]]
- ![[定积分的计算#3. 分部积分法]]

