# 题

![[Pasted image 20240414192115.png]]

# 解

$$
\begin{aligned}
	& A= \lim\limits_{x\to +\infty} \frac{(1+x)^{\frac{3}{2}}}{x^{\frac{3}{2}}}\\
	& = \lim\limits_{x\to +\infty} (1+\frac{1}{x})^{\frac{3}{2}}\\
	& = 1\\\\
	& B= \lim\limits_{x\to +\infty} y-Ax\\
	& = \lim\limits_{x\to +\infty} (1+x) \sqrt[]{1+\frac{1}{x}} -x\\
	& = \lim\limits_{x\to +\infty} 1+ (x) (\sqrt[]{1+\frac{1}{x}} -1)\\
	& = \lim\limits_{x\to +\infty} 1+ x \frac{1}{2}\frac{1}{x}\\
	& = \frac{3}{2}\\\\
	& y= x+ \frac{3}{2}
\end{aligned}
$$
