## 因式分解公式
$$\begin{aligned}
& 1.\ (a\pm b)^2= a^2\pm 2ab+ b^2\\ 
& 2.\ (a\pm b)^3= a^3\pm 3a^2b+ 3ab^2\pm b^3\\ 
& 3.\ a^2-b^2= (a-b)(a+b)\\ 
& 4.\ a^3-b^3= (a-b)(a^2+ ab+ b^2)\\ 
& 5.\ a^3+b^3= (a+b)(a^2- ab+ b^2)\\ 
& 6.\ a^n-b^n= (a-b)(a^{n-1}+a^{n-2}b+ \dots+ ab^{n-2}+ b^{n-1})\\ 
& 7.\ n是正偶数时:\ a^n-b^n= (a-b)(a^{n-1}-a^{n-2}b+ \dots+ ab^{n-2}+ b^{n-1})\\ 
& 8.\ n是正奇数时:\ a^n+b^n= (a-b)(a^{n-1}+a^{n-2}b+ \dots+ ab^{n-2}+ b^{n-1})\\ 
& 9.\ 二项式定理:\\
&\qquad \qquad\begin{equation}
\begin{split}
(a+b)^n &= \sum\limits_{k=0}^{n}C_{n}^{k}a^{n-k}b^k\\\\
&= a^n+ na^{n-1}b+ \frac{n(n-1)}{2!} a^{n-2}b^2+ \dots+ \frac{n(n-1)\dots (n-k+1)}{k!} a^{n-k}b^k+ \dots+ nab^{n-1}+ b^n
\end{split}
\end{equation}
\end{aligned}$$
