# 双曲函数
$$\begin{aligned}
& 1.\ 双曲正弦:\ \mathrm{sh}\ x= \frac{e^x-e^{-x}}{2} \quad (奇)\\
& 2.\ 双曲余弦:\ \mathrm{ch}\ x= \frac{e^x+e^{-x}}{2} \quad (偶)\\
& 3.\ 双曲正切:\ \mathrm{th}\ x= \frac{\mathrm{sh}\ x}{\mathrm{ch}\ x} =\frac{e^x-e^{-x}}{e^x+e^{-x}} (奇)\\
& 4.\ 反双曲正弦:\ \mathrm{arsh}\ x= \ln (x+\sqrt[]{x^2+1}) \quad x\in (-\infty, +\infty) \quad (奇)\\
& 5.\ 反双曲余弦:\ \mathrm{arch}\ x= \ln (x+\sqrt[]{x^2-1}) \quad x\in [1, +\infty]\\
& 6.\ 反双曲正切:\ \mathrm{arth}\ x= \frac{1}{2} \ln\frac{1+x}{1-x} \quad x\in (-1, 1) \quad (奇)\\
\end{aligned}$$

![[双曲函数图像.png]]
![[反双曲函数图像.jpeg]]

## 常用公式
1. $\mathrm{sh}\ (x+y)= \mathrm{sh}\ x\mathrm{ch}\ y+\mathrm{ch}\ x\mathrm{sh}\ y$
2. $\mathrm{sh}\ (x-y)= \mathrm{sh}\ x\mathrm{ch}\ y-\mathrm{ch}\ x\mathrm{sh}\ y$
3. $\mathrm{ch}\ (x+y)= \mathrm{ch}\ x\mathrm{ch}\ y+\mathrm{sh}\ x\mathrm{sh}\ y$
4. $\mathrm{ch}\ (x-y)= \mathrm{ch}\ x\mathrm{ch}\ y-\mathrm{ch}\ x\mathrm{ch}\ y$
5. ${\mathrm{ch}}^2\ x-{\mathrm{sh}}^2\ x=1$
6. $\mathrm{sh}\ 2x=2\mathrm{sh}\ x\mathrm{ch}\ x$
7. $\mathrm{ch}\ 2x=\mathrm{sh}^2\ x+\mathrm{ch}^2\ x$

## 反双曲函数的推导
$$\begin{aligned}
& y=\mathrm{sh}\ x, 由x=\mathrm{sh}\ y, 有x=\frac{e^y-e^{-y}}{2} \\
& 令u= e^y, 则有u^2-2xu-1=0\\
& \therefore u= x\pm \sqrt[]{x^2+1} \\
& \because u=e^y >0\\
& \therefore u= x+\sqrt[]{x^2+1}\\
& \therefore y=\mathrm{arsh}\ x= \ln u= \ln (x+\sqrt[]{x^2+1})\\\\

& y=\mathrm{ch}\ x(x\geqslant 0), 由x=\mathrm{ch}\ y, 有x=\frac{e^y+e^{-y}}{2} >1\\
& 令u= e^y, 则有u^2-2xu+1=0\\
& \therefore u= x\pm \sqrt[]{x^2-1} \\
& \because u=e^y \geqslant 1 (y\geqslant 0)\\
& \therefore u=\ x+\sqrt[]{x^2-1}\\
& \therefore y=\mathrm{arch}\ x= \ln u= \ln (x+\sqrt[]{x^2-1})\\\\

&  {y=\mathrm{th}\ x},由x=\mathrm{th}\ y, 有x=\frac{e^y-e^{-y}}{e^y+e^{-y}}\in (-1, 1)\\
& 令u= e^y, 则有(x-1)u^2+x+1=0\\
& \therefore u= \pm \sqrt[]{\frac{1+x}{1-x}} \\
& \because u=e^y >0 \\
& \therefore u=\sqrt[]{\frac{1+x}{1-x}} \\
& \therefore y=\mathrm{arth}\ x= \ln u= \ln \sqrt[]{\frac{1+x}{1-x}}=\frac{1}{2} \ln\frac{1+x}{1-x}\\
\end{aligned}$$
